src/CSL/Count_Heap.v
@@ -172,6 +172,15 @@ Proof.
   iModIntro. by iExists (GenHeapG L V Σ _ _ γ).
 Qed.
 
+Lemma gen_heap_strong_init `{H: gen_heapPreG L V Σ} σs :
+  (|==> ∃ (H0 : gen_heapG L V Σ) (Hpf: gen_heap_inG = gen_heap_preG_inG), gen_heap_ctx σs ∗
+    own (gen_heap_name _) (◯ (to_gen_heap σs)))%I.
+Proof.
+  iMod (own_alloc (● to_gen_heap σs ⋅ ◯ to_gen_heap σs)) as (γ) "(?&?)".
+  { apply auth_valid_discrete_2; split; auto. exact: to_gen_heap_valid. }
+  iModIntro. unshelve (iExists (GenHeapG L V Σ _ _ γ), _); auto. iFrame.
+Qed.
+
 Section gen_heap.
   Context `{gen_heapG L V Σ}.
   Implicit Types P Q : iProp Σ.
