src/Goose/Proof/RefinementAdequacy.v
@@ -1,0 +1,504 @@
+From iris.algebra Require Import auth gmap frac agree.
+Require Import Helpers.RelationTheorems.
+Require Import Goose.Proof.Interp.
+Require Import Spec.Proc.
+Require Import Spec.ProcTheorems.
+Require Import Spec.Layer.
+From RecoveryRefinement.Goose Require Import Machine GoZeroValues Heap GoLayer.
+Require Export CSL.WeakestPre CSL.Lifting CSL.Adequacy CSL.RefinementAdequacy.
+Import Data.
+Import Filesys.FS.
+Import GoLayer.Go.
+
+
+Class fsPreG (m: GoModel) {wf: GoModelWf m} Σ :=
+  FsPreG {
+      go_fs_dlocks_preG :> Count_Heap.gen_heapPreG string unit Σ;
+      go_fs_dirs_preG :> gen_heapPreG string (gset string) Σ;
+      go_fs_paths_preG :> gen_dirPreG string string (Inode) Σ;
+      go_fs_inodes_preG :> gen_heapPreG Inode (List.list byte) Σ;
+      go_fs_fds_preG :> gen_heapPreG File (Inode * OpenMode) Σ;
+}.
+
+Definition fsΣ (m: GoModel) {wf: GoModelWf m} : gFunctors :=
+  #[gen_heapΣ string (gset string);
+    Count_Heap.gen_heapΣ string unit;
+    gen_dirΣ string string (Inode);
+    gen_heapΣ Inode (List.list byte);
+    gen_heapΣ File (Inode * OpenMode)
+   ].
+
+Instance subG_fsPreG m {wf: GoModelWf m} {Σ} : subG (fsΣ m) Σ → (fsPreG m) Σ.
+Proof. solve_inG. Qed.
+
+Class goosePreG (goose_model: GoModel) {wf: GoModelWf goose_model} Σ := GoosePreG {
+  goose_preG_iris :> invPreG Σ;
+  goose_preG_heap :> Count_Heap.gen_heapPreG (sigT Ptr) (sigT ptrRawModel) Σ;
+  goose_preG_fs :> fsPreG goose_model Σ;
+  goose_preG_treg_inG :> inG Σ (csumR countingR (authR (optionUR (exclR unitC))));
+}.
+
+Definition gooseΣ (m: GoModel) {wf: GoModelWf m} : gFunctors :=
+  #[invΣ; fsΣ m; gen_typed_heapΣ Ptr ptrRawModel;
+      GFunctor (csumR countingR (authR (optionUR (exclR unitC))))].
+Instance subG_goosePreG (m: GoModel) {wf: GoModelWf m} {Σ} : subG (gooseΣ m) Σ → goosePreG m Σ.
+Proof. solve_inG. Qed.
+
+
+Section refinement.
+  Context `{@goosePreG gm gmHwf Σ}.
+  Context OpT (Λa: Layer OpT).
+  Context `{cfgPreG OpT Λa Σ}.
+  Context (impl: LayerImpl GoLayer.Op OpT).
+  Notation compile_op := (compile_op impl).
+  Notation compile_rec := (compile_rec impl).
+  Notation compile_seq := (compile_seq impl).
+  Notation compile := (compile impl).
+  Notation recover := (recover impl).
+  Notation compile_proc_seq := (compile_proc_seq impl).
+  Context (crash_inner: forall {_ : @cfgG OpT Λa Σ} {_: gooseG gm Σ}, iProp Σ).
+  Context (exec_inner: forall {_ : @cfgG OpT Λa Σ} {_ : gooseG gm Σ}, iProp Σ).
+  Context (crash_param: forall (_ : @cfgG OpT Λa Σ) (_ : gooseG gm Σ), Type).
+  Context (crash_inv: forall {H1 : @cfgG OpT Λa Σ} {H2 : gooseG gm Σ}, @crash_param _ _ → iProp Σ).
+  Context (crash_starter: forall {H1 : @cfgG OpT Λa Σ} {H2 : gooseG gm Σ}, @crash_param _ _ → iProp Σ).
+  Context (exec_inv: forall {_ : @cfgG OpT Λa Σ} {_ : gooseG gm Σ}, iProp Σ).
+
+  Context (einv_persist: forall {H1 : @cfgG OpT Λa Σ} {H2 : gooseG gm Σ}, Persistent (exec_inv H1 H2)).
+  Context (cinv_persist: forall {H1 : @cfgG OpT Λa Σ} {H2 : gooseG gm Σ}
+            {P: crash_param _ _}, Persistent (crash_inv H1 H2 P)).
+
+  Context (E: coPset).
+  Context (nameIncl: nclose sourceN ⊆ E).
+  (* TODO: we should get rid of rec_seq if we're not exploiting vertical comp anymore *)
+  Context (recv: proc GoLayer.Op unit).
+  Context (recsingle: recover = rec_singleton recv).
+
+  Context (refinement_op_triples:
+             forall {H1 H2 T1 T2} j K `{LanguageCtx OpT T1 T2 Λa K} (op: OpT T1),
+               j ⤇ K (Call op) ∗ Registered ∗ (@exec_inv H1 H2) ⊢
+                 WP compile (Call op) {{ v, j ⤇ K (Ret v) ∗ Registered }}).
+
+  Context (exec_inv_source_ctx: ∀ {H1 H2}, exec_inv H1 H2 ⊢ source_ctx).
+
+  Lemma refinement_triples:
+             forall {H1 H2 T1 T2} j K `{LanguageCtx OpT T1 T2 Λa K} (e: proc OpT T1),
+               wf_client e →
+               j ⤇ K e ∗ Registered ∗ (@exec_inv H1 H2) ⊢
+                 WP compile e {{ v, j ⤇ K (Ret v) ∗ Registered }}.
+  Proof.
+    intros ???? j K Hctx e Hwf.
+    iIntros "(Hj&Hreg&#Hinv)".
+    iAssert (⌜∃ ea: Layer.State Λa, True⌝)%I as %[? _].
+    {
+      iDestruct (exec_inv_source_ctx with "Hinv") as ((?&?)) "#Hctx".
+      eauto.
+    }
+    assert (Inhabited (Layer.State Λa)).
+    { eexists. eauto. }
+    assert (Inhabited Λa.(OpState)).
+    { eexists. destruct x; eauto. }
+    iInduction e as [] "IH" forall (j T2 K Hctx).
+    - iApply refinement_op_triples; iFrame; eauto.
+    - wp_ret. iFrame.
+    - wp_bind.
+      iApply wp_wand_l. iSplitL ""; last first.
+      * unshelve (iApply ("IH1" $! _ _ _ (fun x => K (Bind x p2)) with "[] Hj"); try iFrame).
+        { eapply Hwf. }
+        { iPureIntro. apply comp_ctx; auto. apply _. }
+      * iIntros (?) "(Hj&Hreg)".
+        iDestruct (exec_inv_source_ctx with "Hinv") as "#Hctx".
+        iMod (ghost_step_bind_ret with "Hj []") as "Hj".
+        { set_solver+. }
+        { eauto. }
+        iApply ("IH" with "[] [] Hj Hreg"); auto.
+        { iPureIntro. eapply Hwf. }
+    - iLöb as "IHloop" forall (init Hwf).
+      iDestruct (exec_inv_source_ctx with "Hinv") as "#Hctx".
+      iMod (ghost_step_loop with "Hj []") as "Hj".
+      { set_solver+. }
+      { eauto. }
+      wp_loop.
+      iApply wp_wand_l.
+      iSplitL ""; last first.
+      * rewrite /loop1. simpl.
+        unshelve (iApply ("IH" $! _ _ _ _ (fun x => K (Bind x
+                               (fun out => match out with
+                               | ContinueOutcome x => Loop body x
+                               | DoneWithOutcome r => Ret r
+                               end))) with "[] Hj Hreg")%proc).
+        { eauto. }
+        { iPureIntro. apply comp_ctx; auto. apply _. }
+      * iIntros (out) "(Hj&Hreg)".
+        destruct out.
+        ** iNext.
+           iMod (ghost_step_bind_ret with "Hj []") as "Hj".
+           { set_solver+. }
+           { eauto. }
+           iApply ("IHloop" with "[] Hj Hreg").
+           { eauto. }
+        ** iNext.
+           iMod (ghost_step_bind_ret with "Hj []") as "Hj".
+           { set_solver+. }
+           { eauto. }
+           wp_ret. iFrame.
+   - inversion Hwf.
+   - inversion Hwf.
+   - iDestruct (exec_inv_source_ctx with "Hinv") as "#Hctx".
+     iMod (ghost_step_spawn with "Hj []") as "(Hj&Hj')".
+     { set_solver+. }
+     { eauto. }
+     iDestruct "Hj'" as (j') "Hj'".
+     iApply (wp_spawn with "Hreg [Hj'] [Hj]").
+     { iNext. iIntros "Hreg'".
+       { wp_bind.
+         iApply (wp_wand with "[Hj' Hreg'] []").
+         { unshelve (iApply ("IH" $! _ _ _ (fun x => Bind x (fun _ => Unregister))
+                               with "[] Hj' Hreg'")).
+           { eauto. }
+           { iPureIntro. apply _. }
+         }
+         { iIntros (?) "(?&?)". iApply (wp_unregister with "[$]"). iIntros "!> ?". eauto. }
+       }
+     }
+     iIntros "!> ?". iFrame.
+  Qed.
+
+  Context (recv_triple:
+             forall {H1 H2} param,
+               (@crash_inv H1 H2 param) ∗ Registered ∗ (@crash_starter H1 H2 param) ⊢
+                    WP recv @ NotStuck; ⊤ {{ v, |={⊤,E}=> ∃ σ2a σ2a', source_state σ2a
+                    ∗ ⌜Proc.crash_step Λa σ2a (Val σ2a' tt)⌝ ∗
+                    ∀ `{Hcfg': cfgG OpT Λa Σ} (Hinv': invG Σ) tr',
+                      source_ctx ∗ source_state σ2a'  ={⊤}=∗
+                      exec_inner Hcfg' (GooseG _ _ Σ Hinv' go_heap_inG go_fs_inG tr')
+                                               }}).
+
+  Context (init_absr: Λa.(OpState) → State → Prop).
+  Context (init_wf: ∀ σ1a σ1c, init_absr σ1a σ1c → dom (gset string) σ1c.(fs).(dirents) =
+                                                   dom (gset string) σ1c.(fs).(dirlocks)).
+
+  Context (init_exec_inner: ∀ σ1a σ1c, init_absr σ1a σ1c →
+      (∀ `{Hex: @gooseG gm gmHwf Σ} `{Hcfg: cfgG OpT Λa Σ},
+          (([∗ map] d ↦ ents ∈ σ1c.(fs).(dirents), d ↦ dom (gset string) ents) ∗
+           source_ctx ∗ source_state σ1a) ={⊤}=∗ exec_inner _ _)).
+
+  (* Helper to update collection of ghost algebra for file system to use new
+     "generation" mapping for fds/dlocks post crash. *)
+  Definition crash_fsG {Σ} (curr: @fsG _ _ Σ) newDirLocks newFds : @fsG _ _ Σ :=
+    FsG _ _ _ newDirLocks (go_fs_dirs_inG) (go_fs_paths_inG) (go_fs_inodes_inG) newFds.
+
+  Context (exec_inv_preserve_crash:
+      (∀ `{Hex: @gooseG gm gmHwf Σ} `{Hcfg: cfgG OpT Λa Σ},
+          exec_inv Hcfg Hex ={⊤, E}=∗ ∀ Hmem' Hdlocks' Hfds' Hreg',
+            (let Hex := GooseG _ _ Σ (go_invG) Hmem' (crash_fsG _ Hdlocks' Hfds') Hreg' in
+           (* TODO: should get dirlocks + uninit global*)
+           True ={E}=∗ crash_inner Hcfg Hex))).
+
+  Context (crash_inv_preserve_crash:
+      (∀ `{Hex: @gooseG gm gmHwf Σ} `{Hcfg: cfgG OpT Λa Σ} param,
+          crash_inv Hcfg Hex param ={⊤, E}=∗ ∀ Hmem' Hdlocks' Hfds' Hreg',
+          (let Hex := GooseG _ _ Σ (go_invG) Hmem' (crash_fsG _ Hdlocks' Hfds') Hreg' in
+           (* TODO: should get dirlocks + uninit global *)
+           True ={E}=∗ crash_inner Hcfg Hex))).
+
+  (* TODO: Much of this business is just to capture the fact that exec_inner/crash_inner
+     should not really mention invariants, because those old invariants are 'dead' *)
+  Context (crash_inner_inv :
+      (∀ `{Hex: @gooseG gm gmHwf Σ} `{Hcfg: cfgG OpT Λa Σ},
+          (∃ Hinv, crash_inner Hcfg (GooseG _ _ Σ Hinv (go_heap_inG) (go_fs_inG) (go_treg_inG))) ∗
+          source_ctx ={⊤}=∗ ∃ param, crash_inv Hcfg Hex param ∗ crash_starter Hcfg Hex param)).
+
+  Context (exec_inner_inv :
+      (∀ `{Hex: @gooseG gm gmHwf Σ} `{Hcfg: cfgG OpT Λa Σ},
+          (∃ Hinv, exec_inner Hcfg (GooseG _ _ Σ Hinv (go_heap_inG) (go_fs_inG) (go_treg_inG))) ∗
+          source_ctx ={⊤}=∗ exec_inv Hcfg Hex)).
+
+  Context (exec_inv_preserve_finish:
+      (∀ `{Hex: @gooseG gm gmHwf Σ} `{Hcfg: cfgG OpT Λa Σ},
+          AllDone -∗ exec_inv Hcfg Hex ={⊤, E}=∗ ∃ (σ2a σ2a' : Λa.(OpState)), source_state σ2a
+          ∗ ⌜Λa.(finish_step) σ2a (Val σ2a' tt)⌝ ∗
+          ∀ `{Hcfg': cfgG OpT Λa Σ} (Hinv': invG Σ) Hmem' Hdlocks' Hfds' Hreg',
+            (let Hex := GooseG _ _ Σ Hinv' Hmem' (crash_fsG _ Hdlocks' Hfds') Hreg' in
+             source_ctx ∗ source_state σ2a' ∗
+            (* TODO: should get fresh global/dirlocks *) True ={⊤}=∗ exec_inner Hcfg' Hex))%I).
+
+
+  Lemma exmach_crash_refinement_seq {T} σ1c σ1a (es: proc_seq OpT T) :
+    init_absr σ1a σ1c →
+    wf_client_seq es →
+    ¬ proc_exec_seq Λa es (rec_singleton (Ret ())) (1, σ1a) Err →
+    ∀ σ2c res, proc_exec_seq GoLayer.Go.l (compile_proc_seq es)
+                                        (rec_singleton recv) (1, σ1c) (Val σ2c res) →
+    ∃ σ2a, proc_exec_seq Λa es (rec_singleton (Ret tt)) (1, σ1a) (Val σ2a res).
+  Proof.
+    rewrite /compile_proc_seq. intros Hinit Hwf_seq Hno_err σ2c0 ?.
+    unshelve (eapply wp_proc_seq_refinement_adequacy with
+                  (Λc := l)
+                  (φ := fun _ _ _ => True%I)
+                  (E0 := E); eauto).
+    clear Hno_err.
+  iAssert (∀ invG H1 ρ, |={⊤}=>
+       ∃ hM hD tR
+         (*
+            (Hmpf_eq : hM.(@gen_heap_inG addr nat Σ nat_eq_dec nat_countable) =
+          H.(@exm_preG_disk Σ).(@gen_heap_preG_inG addr nat Σ nat_eq_dec nat_countable))
+            (Hdpf_eq : hD.(@gen_heap_inG addr nat Σ nat_eq_dec nat_countable) =
+          H.(@exm_preG_disk Σ).(@gen_heap_preG_inG addr nat Σ nat_eq_dec nat_countable))
+          *),
+             ((@state_interp _ _ _ (@gooseG_irisG _ _ _ (GooseG _ _ Σ _ hM hD {| treg_name := tR; treg_counter_inG := _ |}))) (1, σ1c)) ∗
+         (source_ctx' (ρ, σ1a) -∗ source_state σ1a ={⊤}=∗
+         own tR (Cinl (Count (-1))) ∗
+          exec_inner H1 (GooseG _ _ Σ invG hM hD {| treg_name := tR; treg_counter_inG := _ |})))%I
+      as "Hpre".
+  {
+  iIntros.
+  iMod (gen_typed_heap_strong_init (σ1c.(fs).(heap).(allocs))) as (hM Hmpf_eq) "(Hmc&Hm)".
+  iMod (gen_heap_strong_init (fmap (dom (gset string)) (σ1c.(fs).(dirents)))) as (hD Hdpf_eq) "(Hdc&Hd)".
+  iMod (gen_heap_strong_init (σ1c.(fs).(fds))) as (hFDs HFDpf_eq) "(Hfdc&Hfd)".
+  iMod (gen_heap_strong_init (σ1c.(fs).(inodes))) as (hIs HIpf_eq) "(Hidc&Hi)".
+  iMod (gen_dir_strong_init (σ1c.(fs).(dirents))) as (hP HPpf_eq) "(Hpc&Hp)".
+  iMod (Count_Heap.gen_heap_strong_init (λ s, (σ1c.(fs).(dirlocks)) !! s)) as (hL HLpf_eq) "(Hlc&Hl)".
+  iMod (own_alloc (Cinl (Count 0))) as (tR) "Ht".
+  { constructor. }
+  set (tR' := {| treg_name := tR; treg_counter_inG := _ |}).
+  iAssert (own tR (Cinl (Count 1)) ∗ own tR (Cinl (Count (-1))))%I with "[Ht]" as "(Ht&Hreg)".
+  { rewrite /Registered -own_op Cinl_op counting_op' //=. }
+  set (hFG := (FsG _ _ Σ hL hD hP hIs hFDs)).
+  iModIntro. iExists hM, hFG, tR. (* Hmpf_eq, Hdpf_eq. *)
+  iSplitL "Hmc Hdc Hfdc Hidc Hpc Hlc Ht".
+  { iFrame. iPureIntro. eapply init_wf; eauto. }
+  iIntros.
+  iPoseProof (init_exec_inner σ1a σ1c Hinit (GooseG _ _ Σ _ hM hFG tR') _) as "H".
+  iMod ("H" with "[-Hreg]") as "$".
+  { iFrame.  iSplitL "Hd".
+    * iPoseProof (@gen_heap_init_to_bigOp _ _ _ _ _ hD with "[Hd]") as "Hfoo".
+      { by rewrite Hdpf_eq. }
+      by rewrite big_opM_fmap.
+    * iExists _; eauto.
+  }
+  iFrame; eauto.
+  }
+
+  clear Hinit.
+  iInduction es as [|es] "IH" forall (σ1a σ1c) "Hpre"; first by eauto.
+  - iSplit; first by eauto.
+  iExists (fun cfgG s => ∃ (Hex : @gooseG _ _ Σ), state_interp s ∗
+            (∃ hM hDlock' hFds'  tr
+               (*
+               (Hmpf_eq : hM.(@gen_heap_inG addr nat Σ nat_eq_dec nat_countable) =
+                          H.(@exm_preG_disk Σ).(@gen_heap_preG_inG addr nat Σ
+                                                                   nat_eq_dec nat_countable))
+               (Hdpf_eq : (@exm_disk_inG Σ Hex).(@gen_heap_inG addr nat Σ
+                                                               nat_eq_dec nat_countable)=
+                          H.(@exm_preG_disk Σ).(@gen_heap_preG_inG addr nat Σ
+                                                                   nat_eq_dec nat_countable)) 
+                *),
+                gen_typed_heap_ctx ∅ ∗ own tr (Cinl (Count 0))
+                                   ∗ gen_heap_ctx (∅: gmap File (Inode * OpenMode))
+                                   ∗ crash_inner cfgG
+                                   (GooseG _ _ Σ _ hM (crash_fsG (go_fs_inG) hDlock' hFds')
+ {| treg_name := tr; treg_counter_inG := _ |})))%I; auto.
+  iIntros (invG0 Hcfg0).
+  iMod ("Hpre" $! invG0 _ _) as (hM hD tr (* ?? *) ) "(Hstate0&H)".
+  set (tR' := {| treg_name := tr; treg_counter_inG := _ |}).
+  set (hG := (GooseG _ _ Σ _ hM hD tR')).
+  iExists (@state_interp _ _ _ (@gooseG_irisG _ _ _ hG)).
+  (*
+  iExists (@state_interp _ _ _ (@gooseG_irisG _ _ _ hG)).
+   *)
+  iIntros "!> (#Hsrc&Hpt0&Hstate)".
+  iMod ("H" with "Hsrc Hstate") as "(Hreg&Hinv)".
+  iMod (exec_inner_inv hG _ with "[Hinv]") as "#Hinv".
+  { iSplitR ""; last by (iExists _; iFrame). iExists _. iFrame. }
+  simpl.
+  iModIntro.
+  iFrame "Hstate0".
+  iSplitL "Hpt0 Hreg".
+  {  iPoseProof (@wp_mono with "[Hpt0 Hreg]") as "H"; swap 1 2.
+     { iApply refinement_triples. destruct (Hwf_seq) as (?&?). eauto. iFrame. iFrame "Hinv".
+     }
+     { reflexivity. }
+     rewrite /compile_whole.
+     wp_bind.
+     iApply (wp_wand with "H [Hinv]").
+     iIntros (v) "(Hpt0&Hreg)". iFrame.
+     wp_bind.
+     iApply (wp_wait with "Hreg").
+     iIntros "!> Hdone".
+     wp_ret. iFrame. iIntros (σ2c) "Hmach".
+     iMod (exec_inv_preserve_finish with "Hdone Hinv") as (σ2a σ2a') "(H&Hfina&Hfinish)".
+     iDestruct "Hfina" as %Hfina.
+     iModIntro. iExists _; iFrame; auto.
+     rewrite -/wp_proc_seq_refinement.
+     iIntros (σ2c'). iIntros.
+     unshelve (iExists σ2a', _); [eauto |]; [].
+     iApply "IH".
+     { iPureIntro. destruct Hwf_seq. eauto. }
+     { iIntros.
+       destruct σ2c as (n&σ2c). iDestruct "Hmach" as "(?&Hmach)".
+       iMod (gen_typed_heap_strong_init ∅) as (hM' Hmpf_eq') "(Hmc&Hm)".
+       iMod (gen_heap_strong_init (∅: gmap File (Inode * OpenMode)))
+         as (hFds' Hfds'_eq') "(Hfdsc&Hfd)".
+       iMod (Count_Heap.gen_heap_strong_init 
+               (λ s, ((λ _ : LockStatus * (), (Unlocked, ())) <$> σ2c.(fs).(dirlocks)) !! s))
+         as (hDlocks' Hdlocks'_eq') "(Hdlocksc&Hlocks)".
+       iMod (own_alloc (Cinl (Count 0))) as (tR_fresh') "Ht".
+       { constructor. }
+       iAssert (own tR_fresh' (Cinl (Count 1))
+                    ∗ own tR_fresh' (Cinl (Count (-1))))%I with "[Ht]" as "(Ht&Hreg)".
+       { rewrite /Registered -own_op Cinl_op counting_op' //=. }
+       set (tR''' := {| treg_name := tR_fresh'; treg_counter_inG := _ |}).
+       iModIntro.
+       iExists hM'. iExists (crash_fsG hD hDlocks' hFds'). iExists tR_fresh'.
+       (* unshelve (iExists _, _); try eauto. *)
+       iFrame.
+       iSplitL ("Hmc Hmach Hfdsc Hdlocksc").
+       { iClear "IH".
+         iDestruct "Hmach" as "(?&?&?&?&?&?&?)".
+         repeat deex. inv_step.
+         rewrite H4. simpl.
+         iFrame. simpl.
+         rewrite dom_fmap_L.
+         iFrame.
+       }
+       iIntros "Hctx' Hsrc'". iMod ("Hfinish" $! _ _ hM' with "[-]").
+       iSplitL "Hctx'"; first by (iExists _; iFrame). iFrame.
+       unfold hG. simpl. unfold tR'''. iFrame.
+       eauto.
+     }
+  }
+  iSplit.
+  { iIntros (σ2c) "Hmach".
+    destruct σ2c as (n&σ2c). iDestruct "Hmach" as "(?&Hmach)".
+    iMod (exec_inv_preserve_crash with "Hinv") as "Hinv_post".
+    iMod (gen_typed_heap_strong_init ∅) as (hM' Hmpf_eq') "(Hmc&Hm)".
+    iMod (gen_heap_strong_init (∅: gmap File (Inode * OpenMode)))
+      as (hFds' Hfds'_eq') "(Hfdsc&Hfd)".
+    iMod (Count_Heap.gen_heap_strong_init 
+            (λ s, ((λ _ : LockStatus * (), (Unlocked, ())) <$> σ2c.(fs).(dirlocks)) !! s))
+      as (hDlocks' Hdlocks'_eq') "(Hdlocksc&Hlocks)".
+    iMod (own_alloc (Cinl (Count 0))) as (tR_fresh') "Ht".
+    { constructor. }
+    set (tR''' := {| treg_name := tR_fresh'; treg_counter_inG := _ |}).
+    iMod ("Hinv_post" with "[Hm]") as "Hinv'".
+    auto.
+    iIntros. iModIntro.
+    unfold hG.
+    simpl.
+
+
+    iExists (GooseG _ _ Σ (@go_invG _ _ _ hG) hM hD tR'). iFrame.
+    iExists hM', _, _, tR_fresh'. iFrame.
+  }
+  iClear "Hsrc".
+  iModIntro. iIntros (invG Hcfg' ?? Hcrash) "(Hinv0&#Hsrc)".
+  iDestruct "Hinv0" as (HexmachG') "(Hinterp&Hinv0)".
+  iDestruct "Hinv0" as (hM' hDl' hFd' tR_fresh' (* Hmpf_eq' Hmdpf_eq' *)) "(Hmc'&Hreg&Hfdc'&Hcrash_inner)".
+  iClear "Hinv".
+  set (tR''' := {| treg_name := tR_fresh'; treg_counter_inG := _ |}).
+  iMod (crash_inner_inv (GooseG _ _ Σ _
+                                 hM' (crash_fsG (go_fs_inG) hDl' hFd') tR''') Hcfg'
+                         with "[Hcrash_inner]") as (param) "(#Hinv&Hstarter)".
+  { iIntros. simpl. iSplitR ""; last by (iExists _; iFrame).
+    iExists (gooseG_irisG.(@iris_invG GoLayer.Op (Layer.State l) Σ)). iFrame. }
+  iModIntro.
+  iAssert (own tR_fresh' (Cinl (Count 1)) ∗ own tR_fresh' (Cinl (Count (-1))))%I
+    with "[Hreg]" as "(Ht&Hreg)".
+  { rewrite /Registered -own_op Cinl_op counting_op' //=. }
+  iExists (@state_interp _ _ _ (@gooseG_irisG _ _ _ (GooseG _ _ _ _ hM' (crash_fsG (@go_fs_inG _ _ _ HexmachG') hDl' hFd') tR'''))).
+  (*
+  iExists (@state_interp _ _ _ (@gooseG_irisG _ _ tR''' hG)).
+   *)
+  (*
+  iExists (@ex_mach_interp Σ hM' (exm_disk_inG) tR''').
+   *)
+  iSplitL "Hinterp Ht Hmc' Hfdc'".
+  { (* shows ex_mach_interp is holds after crash for next gen *)
+    destruct a, a0.
+    iDestruct "Hinterp" as "(?&Hinterp)".
+    destruct Hcrash as ([]&(?&?)&Hput&Hrest).
+    inversion Hput. subst. inv_step.
+    inversion Hrest; subst. inversion H1. subst.
+    deex. inv_step.
+    inv_step. inversion H2. inv_step. inversion H3. subst.
+    inv_step. subst.
+    inversion H4. subst. deex. inv_step. subst.
+    rewrite H6.
+    simpl.
+    iSplitL "Ht".
+    { iFrame. }
+    iFrame.
+    simpl.
+    iFrame.
+    unfold RecordSet.set. simpl.
+    iDestruct "Hinterp" as "(?&?&?&?&?&?&?)".
+    unfold crash_fsG. simpl. unfold fs_interp. simpl.
+    iFrame.
+    iSplitL "".
+    { (* todo: need to include dirlocks in the invariant, but to do that
+         we have to keep track of what directories there are throughout *)
+      admit. }
+    rewrite dom_fmap_L. auto.
+  }
+  iSplitL "Hinv Hreg Hstarter".
+  {
+    iPoseProof (@wp_mono with "[Hinv Hreg Hstarter IH]") as "H"; swap 1 2.
+    { iApply recv_triple. iFrame "Hstarter". iFrame. iApply "Hinv". }
+    { reflexivity. }
+    iApply (@wp_wand with "H [IH]").
+    iIntros (_) "H". iIntros (σ2c) "Hinterp".
+    iMod "H". iModIntro.
+    iDestruct "H" as (σ2a σ2a') "(Hsource&Hinner&Hfinish)".
+    iExists (1, σ2a), (1, σ2a'). iFrame.
+     rewrite -/wp_proc_seq_refinement.
+     iDestruct "Hinner" as %?.
+     iSplitL "".
+     { iPureIntro. exists tt, (1, σ2a); split; eauto. econstructor. split; eauto. eauto.
+       econstructor; eauto.
+     }
+     iApply "IH".
+     { destruct Hwf_seq. eauto. }
+     { iIntros.
+       iMod (@own_alloc _ _ H.(@goose_preG_treg_inG gm gmHwf Σ)
+                        (Cinl (Count 0))) as (tR_fresh'') "Ht".
+       { constructor. }
+       iAssert (@own _ _ H.(@goose_preG_treg_inG gm gmHwf Σ) tR_fresh'' (Cinl (Count 1))
+                    ∗ @own _ _ H.(@goose_preG_treg_inG gm gmHwf Σ) tR_fresh'' (Cinl (Count (-1))))%I with "[Ht]" as "(Ht&Hreg)".
+       { rewrite /Registered -own_op Cinl_op counting_op' //=. }
+       set (tR'''' := {| treg_name := tR_fresh''; treg_counter_inG := H.(@goose_preG_treg_inG gm gmHwf Σ) |}).
+       iModIntro.
+       iExists hM'.
+       iExists (crash_fsG (HexmachG'.(@go_fs_inG _ _ Σ)) hDl' hFd'). iExists tR_fresh''.
+       destruct σ2c.
+       iDestruct "Hinterp" as "(?&?&?&?&?&?&?&?)".
+       iFrame. iIntros.
+       iFrame.
+       iMod ("Hfinish" with "[-]"). iSplitL ""; first by (iExists _; iFrame).
+       iFrame. simpl. unfold tR''''. eauto.
+     }
+  }
+  {
+    iIntros (σ2c) "Hmach".
+    destruct σ2c as (n&σ2c). iDestruct "Hmach" as "(?&Hmach)".
+    iMod (crash_inv_preserve_crash with "Hinv") as "Hinv_post".
+    iMod (gen_typed_heap_strong_init ∅) as (hM'' Hmpf_eq'') "(Hmc&Hm)".
+    iMod (gen_heap_strong_init (∅: gmap File (Inode * OpenMode)))
+      as (hFds' Hfds'_eq') "(Hfdsc&Hfd)".
+    iMod (Count_Heap.gen_heap_strong_init
+            (λ s, ((λ _ : LockStatus * (), (Unlocked, ())) <$> σ2c.(fs).(dirlocks)) !! s))
+      as (hDlocks' Hdlocks'_eq') "(Hdlocksc&Hlocks)".
+    iMod (own_alloc (Cinl (Count 0))) as (tR_fresh'') "Ht".
+    { constructor. }
+    set (tR'''' := {| treg_name := tR_fresh''; treg_counter_inG := _ |}).
+    iMod ("Hinv_post" with "[Hm]") as "Hinv'".
+    { eauto. }
+    iIntros. iModIntro.
+    unfold hG.
+    simpl.
+    iDestruct "Hmach" as "(?&?&?&?&?&?&?)".
+    iExists (GooseG _ _ Σ invG hM'
+               (crash_fsG HexmachG'.(@go_fs_inG _ _ Σ) hDl' hFd') tR'''). iFrame.
+    iExists hM'', _, _, tR_fresh''. iFrame.
+  Admitted.
+
+End refinement.
